More definitions for general propositional logic.

PropositionalLogic/ClassicalPropositionalLogic.v
@@ -3,16 +3,36 @@ Require Import Logic.PropositionalLogic.Syntax.
 
 Local Open Scope PropositionalLogic.
 
-Section ClassicalPropositionalLogic.
+Section ClassicalPropositionalLogicSection.
 
-Context {Var: Type}.
+Context {L: PropositionalLanguage}.
 
-Definition reduce: expr Var -> expr Var -> Prop :=
-  syntax_reduce
-   (fun x y =>
-      ImpNegAsPrime.atomic_reduce x y \/
-      ReduceIff.atomic_reduce x y \/
-      ReduceTrueFalse.atomic_reduce x y).
+Definition reduce: relation expr:=
+  clos_refl_trans _
+   (prop_congr
+     (relation_disjunction
+        ImpNegAsPrime.atomic_reduce
+        (relation_disjunction
+          ReduceIff.atomic_reduce
+          ReduceTrueFalse.atomic_reduce))).
+
+Class ClassicalPropositionalLogic := {
+  provable: expr -> Prop;
+  syntactic_reduction_rule: forall x y, reduce x y -> provable x -> provable y;
+  modus_ponens: forall x y, provable (x --> y) -> provable x -> provable y;
+  axiom1: forall x y, provable (x --> (y --> x));
+  axiom2: forall x y z, provable ((x --> y --> z) --> (x --> y) --> (x --> z));
+  axiom3: forall x y, provable ((~~ y --> x) --> (~~ y --> ~~ x) --> y)
+}.
+
+Instance ClassicalPropositionalLogic_ProofTheory (Gamma: ClassicalPropositionalLogic):
+  ProofTheory (PropositionalLanguage_Language L) :=
+  AxiomaticProofTheory_ProofTheory
+   (AxiomaticProofTheory.Build_ProofTheory (PropositionalLanguage_Language L) provable).
+
+End ClassicalPropositionalLogicSection.
+
+Module ClassicalPropositionalLogic.
 
 Inductive provable: expr Var -> Prop :=
 | syntactic_reduction_rule: forall x y, reduce x y -> provable x -> provable y
