PropositionalLogic/Syntax.v
@@ -1,4 +1,37 @@
+Require Export Coq.Relations.Relation_Definitions.
+Require Export Coq.Relations.Relation_Operators.
+Require Export Coq.Relations.Relation_Definitions.
+Require Export Coq.Classes.RelationClasses.
 Require Import Logic.LogicBase.
+
+Class PropositionalLanguage: Type := {
+  expr: Type;
+  andp : expr -> expr -> expr;
+  orp : expr -> expr -> expr;
+  imp : expr -> expr -> expr;
+  iffp : expr -> expr -> expr;
+  negp : expr -> expr;
+  truep : expr;
+  falsep : expr
+}.
+
+Instance PropositionalLanguage_Language (L: PropositionalLanguage): Language :=
+  Build_Language expr.
+
+Instance PropositionalLanguage__nLanguage (L: PropositionalLanguage):  NormalLanguage _ :=
+  Build_NormalLanguage (PropositionalLanguage_Language L) falsep imp.
+
+Notation "x && y" := (andp x y) (at level 40, left associativity) : PropositionalLogic.
+Notation "x || y" := (orp x y) (at level 50, left associativity) : PropositionalLogic.
+Notation "x --> y" := (imp x y) (at level 55, right associativity) : PropositionalLogic.
+Notation "x <--> y" := (iffp x y) (at level 60, no associativity) : PropositionalLogic.
+Notation "~~ x" := (negp x) (at level 35) : PropositionalLogic.
+Notation "'FF'" := falsep : PropositionalLogic.
+Notation "'TT'" := truep : PropositionalLogic.
+
+Local Open Scope PropositionalLogic.
+
+Module PropositionalLanguage.
 
 Inductive expr {Var: Type}: Type :=
   | andp : expr -> expr -> expr
@@ -12,37 +45,27 @@ Inductive expr {Var: Type}: Type :=
 
 Implicit Arguments expr.
 
-Notation "x && y" := (andp x y) (at level 40, left associativity) : PropositionalLogic.
-Notation "x || y" := (orp x y) (at level 50, left associativity) : PropositionalLogic.
-Notation "x --> y" := (imp x y) (at level 55, right associativity) : PropositionalLogic.
-Notation "x <--> y" := (iffp x y) (at level 60, no associativity) : PropositionalLogic.
-Notation "~~ x" := (negp x) (at level 35) : PropositionalLogic.
-Notation "'FF'" := falsep : PropositionalLogic.
-Notation "'TT'" := truep : PropositionalLogic.
+Instance PropositionalLanguage (Var: Type): PropositionalLanguage :=
+  Build_PropositionalLanguage (expr Var) andp orp imp iffp negp truep falsep.
 
-Local Open Scope PropositionalLogic.
+End PropositionalLanguage.
 
-Instance PropositionalLanguage (Var: Type): Language := Build_Language (expr Var).
-
-Instance nPropositionalLanguage (Var: Type): NormalLanguage (PropositionalLanguage Var) :=
-  Build_NormalLanguage (PropositionalLanguage Var) FF imp.
-
-Inductive syntax_reduce {Var: Type} {atomic_reduce: expr Var -> expr Var -> Prop}:  expr Var -> expr Var -> Prop :=
-| atomic_step: forall x y, atomic_reduce x y -> syntax_reduce x y
-| reduce_refl: forall x, syntax_reduce x x
-| reduce_trans: forall x y z, syntax_reduce x y -> syntax_reduce y z -> syntax_reduce x z
-| andp_congr: forall x1 x2 y1 y2, syntax_reduce x1 y1 -> syntax_reduce x2 y2 -> syntax_reduce (x1 && x2) (y1 && y2)
-| orp_congr: forall x1 x2 y1 y2, syntax_reduce x1 y1 -> syntax_reduce x2 y2 -> syntax_reduce (x1 || x2) (y1 || y2)
-| imp_congr: forall x1 x2 y1 y2, syntax_reduce x1 y1 -> syntax_reduce x2 y2 -> syntax_reduce (x1 --> x2) (y1 --> y2)
-| iffp_congr: forall x1 x2 y1 y2, syntax_reduce x1 y1 -> syntax_reduce x2 y2 -> syntax_reduce (x1 <--> x2) (y1 <--> y2)
-| negp_congr: forall x y, syntax_reduce x y -> syntax_reduce (~~ x) (~~ y)
+Inductive prop_congr {L: PropositionalLanguage} {atomic_reduce: relation expr}: relation expr :=
+| atomic_step: forall x y, atomic_reduce x y -> prop_congr x y
+| andp_congr: forall x1 x2 y1 y2, prop_congr x1 y1 -> prop_congr x2 y2 -> prop_congr (x1 && x2) (y1 && y2)
+| orp_congr: forall x1 x2 y1 y2, prop_congr x1 y1 -> prop_congr x2 y2 -> prop_congr (x1 || x2) (y1 || y2)
+| imp_congr: forall x1 x2 y1 y2, prop_congr x1 y1 -> prop_congr x2 y2 -> prop_congr (x1 --> x2) (y1 --> y2)
+| iffp_congr: forall x1 x2 y1 y2, prop_congr x1 y1 -> prop_congr x2 y2 -> prop_congr (x1 <--> x2) (y1 <--> y2)
+| negp_congr: forall x y, prop_congr x y -> prop_congr (~~ x) (~~ y)
 .
 
-Arguments syntax_reduce {Var} atomic_reduce _ _.
+(* Locate clos_refl_trans. *)
+
+Arguments prop_congr {L} atomic_reduce _ _.
 
 Module ImpNegAsPrime.
 
-Inductive atomic_reduce {Var: Type}: expr Var -> expr Var -> Prop :=
+Inductive atomic_reduce {L: PropositionalLanguage}: expr -> expr -> Prop :=
 | andp_reduce: forall x y, atomic_reduce (x && y) (~~ (x --> ~~ y))
 | orp_reduce: forall x y, atomic_reduce (x || y) (~~ x --> y)
 .
@@ -51,7 +74,7 @@ End ImpNegAsPrime.
 
 Module ImpAndOrAsPrime.
 
-Inductive atomic_reduce {Var: Type}: expr Var -> expr Var -> Prop :=
+Inductive atomic_reduce {L: PropositionalLanguage}: expr -> expr -> Prop :=
 | negp_reduce: forall x, atomic_reduce (~~ x) (x --> FF)
 .
 
@@ -59,14 +82,14 @@ End ImpAndOrAsPrime.
 
 Module ReduceIff.
 
-Inductive atomic_reduce {Var: Type}: expr Var -> expr Var -> Prop :=
+Inductive atomic_reduce {L: PropositionalLanguage}: expr -> expr -> Prop :=
 | iff_reduce: forall x y, atomic_reduce (x <--> y) ((x --> y) && (y --> x)).
 
 End ReduceIff.
 
 Module ReduceTrueFalse.
 
-Inductive atomic_reduce {Var: Type}: expr Var -> expr Var -> Prop :=
+Inductive atomic_reduce {L: PropositionalLanguage}: expr -> expr -> Prop :=
 | falsep_reduce: atomic_reduce FF (~~ TT)
 | truep_reduce: forall x, atomic_reduce TT (x --> x).
 
